add nda_h_final and nda_h_bottom lemma

automat/ndAutomaton.thy
@@ -57,9 +57,12 @@ lift_definition ndaRan :: "('s, 'm::message) ndAutomaton \<rightarrow> channel s
 
 
   (* Only monofun, not cont *)
-definition ndaToDo:: "channel set \<Rightarrow> channel set \<Rightarrow> ('s \<times> 'm::message SB) set rev \<Rightarrow> ('s \<Rightarrow> 'm SPS) \<Rightarrow> 'm SPS" where
-"ndaToDo In Out S \<equiv> \<lambda> h. uspecFlatten In Out 
+definition ndaConcOutFlatten:: "channel set \<Rightarrow> channel set \<Rightarrow> ('s \<times> 'm::message SB) set rev \<Rightarrow> ('s \<Rightarrow> 'm SPS) \<Rightarrow> 'm SPS" where
+"ndaConcOutFlatten In Out S \<equiv> \<lambda> h. uspecFlatten In Out 
                 (setrevImage (\<lambda>(state, sb). spsConcOut sb\<cdot>(h state)) S)"
+
+definition uspecIsStrict :: "'a::ubcl_comp ufun uspec \<Rightarrow> bool" where
+"uspecIsStrict = uspecForall ufIsStrict"
 
 (* ----------------------------------------------------------------------- *)
  section \<open>Lemma\<close>
@@ -74,13 +77,13 @@ lemma nddom_finite[simp]:  "finite (ndaDom\<cdot>nda)"
   by (smt Rep_ndAutomaton fst_conv mem_Collect_eq ndaDom.abs_eq 
       ndaDom.rep_eq ndaWell.elims(2) snd_conv undiscr_Discr)
 
-lemma ndatodo_monofun: "monofun (ndaToDo In Out S)" (is "monofun ?f")
+lemma ndatodo_monofun: "monofun (ndaConcOutFlatten In Out S)" (is "monofun ?f")
 proof (rule monofunI)                 
   fix x y :: "'a \<Rightarrow> 'b SPS"
   assume "x \<sqsubseteq> y"
   hence h: "(\<lambda>(state, sb). spsConcOut sb\<cdot>(x state)) \<sqsubseteq> (\<lambda>(state, sb). spsConcOut sb\<cdot>(y state))"
     by (simp add: below_fun_def cont_pref_eq1I) 
-  thus "?f x \<sqsubseteq> ?f y" by (metis (no_types) h monofun_def ndaToDo_def uspecflatten_image_monofun)
+  thus "?f x \<sqsubseteq> ?f y" by (metis (no_types) h monofun_def ndaConcOutFlatten_def uspecflatten_image_monofun)
  qed
 
 
@@ -92,32 +95,32 @@ proof -
     by (metis (no_types, lifting) b0 monofun_def uspecflatten_monofun)
 qed
 
-lemma ndatodo_monofun3: "S1 \<sqsubseteq> S2 \<Longrightarrow> h1 \<sqsubseteq> h2 \<Longrightarrow> (ndaToDo In Out S1 h1) \<sqsubseteq> (ndaToDo In Out S2 h2)"
+lemma ndatodo_monofun3: "S1 \<sqsubseteq> S2 \<Longrightarrow> h1 \<sqsubseteq> h2 \<Longrightarrow> (ndaConcOutFlatten In Out S1 h1) \<sqsubseteq> (ndaConcOutFlatten In Out S2 h2)"
 proof -
   assume a1: "h1 \<sqsubseteq> h2"
   assume "S1 \<sqsubseteq> S2"
   then have "uspecFlatten In Out (setrevImage (\<lambda>(a, u). spsConcOut u\<cdot>(h1 a)) S1) \<sqsubseteq> uspecFlatten In Out (setrevImage (\<lambda>(a, u). spsConcOut u\<cdot>(h1 a)) S2)"
     by (metis (no_types) monofun_def ndatodo_monofun2)
   then show ?thesis
-    using a1 by (metis (no_types) HOLCF_trans_rules(1) monofun_def ndaToDo_def ndatodo_monofun)
+    using a1 by (metis (no_types) HOLCF_trans_rules(1) monofun_def ndaConcOutFlatten_def ndatodo_monofun)
 qed
 
 
 
 definition ndaHelper2:: "channel set \<Rightarrow> channel set \<Rightarrow> 
   's \<Rightarrow> (('s \<times>'e) \<Rightarrow> ('s \<times> 'm::message SB) set rev) \<Rightarrow> ('s \<Rightarrow> 'm SPS) \<Rightarrow> ('e \<Rightarrow> 'm SPS)" where
-"ndaHelper2 In Out s transition \<equiv> \<lambda> h. (\<lambda>e. ndaToDo In Out (transition (s,e)) h)"
+"ndaHelper2 In Out s transition \<equiv> \<lambda> h. (\<lambda>e. ndaConcOutFlatten In Out (transition (s,e)) h)"
 
 
 lemma ndaHelper2_monofun: "monofun (ndaHelper2 In Out s transition)"
   unfolding ndaHelper2_def
-  by (metis (mono_tags, lifting) mono2mono_lambda monofun_def ndaToDo_def ndatodo_monofun)
+  by (metis (mono_tags, lifting) mono2mono_lambda monofun_def ndaConcOutFlatten_def ndatodo_monofun)
 
 lemma ndaHelper2_monofun2: "monofun (ndaHelper2 In Out s)"
   unfolding ndaHelper2_def
   apply(rule monofunI)
   apply(auto simp add: below_fun_def)
-  by (metis (mono_tags, lifting) monofun_def ndaToDo_def ndatodo_monofun2)
+  by (metis (mono_tags, lifting) monofun_def ndaConcOutFlatten_def ndatodo_monofun2)
 
 definition nda_h_inner::"('s::type, 'm::message) ndAutomaton \<Rightarrow> ('s \<Rightarrow> 'm SPS) \<Rightarrow> ('s \<Rightarrow> 'm SPS)" where
 "nda_h_inner nda h \<equiv>  let dom = (ndaDom\<cdot>nda);
@@ -146,7 +149,7 @@ lemma ndaran_below_eq:"nda1 \<sqsubseteq> nda2 \<Longrightarrow> ndaRan\<cdot>nd
   by (metis (mono_tags, hide_lams) below_ndAutomaton_def discrete_cpo snd_monofun)
 
 lemma nda_helper2_h2:"x\<sqsubseteq>y \<Longrightarrow> ndaHelper2 CS1 CS2 xb x xa \<sqsubseteq> ndaHelper2 CS1 CS2 xb y xa"
-  by (metis (mono_tags, lifting) below_fun_def monofun_def ndaHelper2_def ndaToDo_def ndatodo_monofun2)
+  by (metis (mono_tags, lifting) below_fun_def monofun_def ndaHelper2_def ndaConcOutFlatten_def ndatodo_monofun2)
 
 lemma nda_h_inner_monofun2: "monofun (nda_h_inner)"
   unfolding nda_h_inner_def
@@ -183,7 +186,7 @@ lemma nda_h_valid_domain: "(SetPcpo.setify (\<lambda>a. USPEC (ndaDom\<cdot>nda)
   using nda_h_valid_domain_h by fastforce
 
 lemma nda_h_fixpoint:"nda_h nda = nda_h_inner nda (nda_h nda)"
-  by (metis (no_types) nddom_finite lfp_fix nda_h_def nda_h_inner_monofun nda_h_valid_domain nda_inner_good)
+  by (metis (no_types) lfp_fix nda_h_def nda_h_inner_monofun nda_h_valid_domain nda_inner_good)
 
 lemma nda_h_mono:  "monofun nda_h"
   apply(rule monofunI)
@@ -196,7 +199,7 @@ lemma nda_h_mono:  "monofun nda_h"
 
 
 definition nda_H :: "('s, 'm::message) ndAutomaton \<Rightarrow> 'm SPS" where
-"nda_H nda \<equiv> ndaToDo (ndaDom\<cdot>nda)(ndaRan\<cdot>nda) (ndaInitialState\<cdot>nda) (nda_h nda)" 
+"nda_H nda \<equiv> ndaConcOutFlatten (ndaDom\<cdot>nda)(ndaRan\<cdot>nda) (ndaInitialState\<cdot>nda) (nda_h nda)" 
 
 
 lemma "cont (\<lambda>nda. fst (Rep_ndAutomaton nda))"
@@ -224,5 +227,13 @@ shows "nda1 \<sqsubseteq> nda2"
    apply (metis Discr_undiscr)+
   done
 
+
+lemma nda_h_final: assumes "sbedom sbe = ndaDom\<cdot>nda"
+  shows "spsConcIn (sbe2SB sbe) (nda_h nda state) = 
+  uspecFlatten (ndaDom\<cdot>nda) (ndaRan\<cdot>nda) (setrevImage (\<lambda>(s, sb). spsConcOut sb\<cdot>(nda_h nda s)) ((ndaTransition\<cdot>nda) (s,sbe)))"
+  sorry
+
+lemma nda_h_bottom: "uspecIsStrict (nda_h nda state)"
+  sorry
 
 end
